Minor work on translation proofs (#48)
* Towards translation proofs

* Fix

* Another fix

Cpc/Spec.lean
@@ -329,7 +329,7 @@ def __eo_to_smt : Term -> SmtTerm
   | (Term.Apply (Term.Apply (Term.UOp UserOp.str_in_re) x1) x2) => (SmtTerm.str_in_re (__eo_to_smt x1) (__eo_to_smt x2))
   | (Term.Apply (Term.UOp UserOp.seq_unit) x1) => (SmtTerm.seq_unit (__eo_to_smt x1))
   | (Term.Apply (Term.Apply (Term.UOp UserOp.seq_nth) x1) x2) => (SmtTerm.seq_nth (__eo_to_smt x1) (__eo_to_smt x2))
-  | (Term.Apply (Term.Apply (Term.Apply (Term.UOp UserOp._at_re_unfold_pos_component) x1) x2) x3) => (native_ite (native_teq (__eo_is_neg x3) (Term.Boolean false)) (__eo_to_smt_re_unfold_pos_component (__eo_to_smt x1) (__eo_to_smt x2) (__eo_to_smt_nat x3)) SmtTerm.None)
+  | (Term.Apply (Term.Apply (Term.Apply (Term.UOp UserOp._at_re_unfold_pos_component) x1) x2) x3) => (native_ite (native_teq (__eo_is_z x3) (Term.Boolean true)) (native_ite (native_teq (__eo_is_neg x3) (Term.Boolean false)) (__eo_to_smt_re_unfold_pos_component (__eo_to_smt x1) (__eo_to_smt x2) (__eo_to_smt_nat x3)) SmtTerm.None) SmtTerm.None)
   | (Term.Apply (Term.Apply (Term.UOp UserOp._at_strings_deq_diff) x1) x2) => 
     let _v0 := (SmtTerm.Numeral 1)
     let _v2 := (SmtTerm.Var "_at_x" SmtType.Int)
@@ -377,7 +377,7 @@ def __eo_to_smt : Term -> SmtTerm
   | (Term.Apply (Term.UOp UserOp._at_div_by_zero) x1) => (SmtTerm.qdiv (__eo_to_smt x1) (SmtTerm.Rational (native_mk_rational 0 1)))
   | (Term.Apply (Term.Apply (Term.UOp UserOp.forall) x1) x2) => (SmtTerm.not (__eo_to_smt_exists x1 (SmtTerm.not (__eo_to_smt x2))))
   | (Term.Apply (Term.Apply (Term.UOp UserOp.exists) x1) x2) => (__eo_to_smt_exists x1 (__eo_to_smt x2))
-  | (Term._at_quantifiers_skolemize (Term.Apply (Term.Apply (Term.UOp UserOp.forall) x1) x2) x3) => (native_ite (native_teq (__eo_is_neg x3) (Term.Boolean false)) (__eo_to_smt_quantifiers_skolemize (__eo_to_smt_exists x1 (SmtTerm.not (__eo_to_smt x2))) (__eo_to_smt_nat x3)) SmtTerm.None)
+  | (Term._at_quantifiers_skolemize (Term.Apply (Term.Apply (Term.UOp UserOp.forall) x1) x2) x3) => (native_ite (native_teq (__eo_is_z x3) (Term.Boolean true)) (native_ite (native_teq (__eo_is_neg x3) (Term.Boolean false)) (__eo_to_smt_quantifiers_skolemize (__eo_to_smt_exists x1 (SmtTerm.not (__eo_to_smt x2))) (__eo_to_smt_nat x3)) SmtTerm.None) SmtTerm.None)
   | (Term.Apply (Term.Apply (Term.UOp UserOp.int_to_bv) x1) x2) => (SmtTerm.int_to_bv (__eo_to_smt x1) (__eo_to_smt x2))
   | (Term.Apply (Term.UOp UserOp.ubv_to_int) x1) => (SmtTerm.ubv_to_int (__eo_to_smt x1))
   | (Term.Apply (Term.UOp UserOp.sbv_to_int) x1) => (SmtTerm.sbv_to_int (__eo_to_smt x1))
